generational/spec/GC.Gen.PromotionDemand.fst
@@ -1,0 +1,90 @@
+/// ---------------------------------------------------------------------------
+/// GC.Gen.PromotionDemand -- Conservative minor-promotion allocation demand
+/// ---------------------------------------------------------------------------
+
+module GC.Gen.PromotionDemand
+
+open FStar.Seq
+
+module U64 = FStar.UInt64
+
+open GC.Gen.MinorHeap
+
+module MultiAlloc = GC.Spec.MajorAllocator.MultiAlloc
+
+let rec minor_promotion_requests_from
+  (minor: minor_state) (objs: seq U64.t) (idx: nat)
+  : GTot (list nat)
+  (decreases (Seq.length objs - idx))
+  =
+  if idx >= Seq.length objs then []
+  else
+    minor_wosize minor (Seq.index objs idx) ::
+    minor_promotion_requests_from minor objs (idx + 1)
+
+let minor_promotion_requests (minor: minor_state) : GTot (list nat) =
+  minor_promotion_requests_from minor (minor_objects minor) 0
+
+let minor_promotion_demand (minor: minor_state) : GTot nat =
+  MultiAlloc.allocation_list_demand (minor_promotion_requests minor)
+
+let minor_promotion_demand_eq (minor: minor_state)
+  : Lemma
+      (ensures
+        minor_promotion_demand minor ==
+        MultiAlloc.allocation_list_demand (minor_promotion_requests minor))
+  = ()
+
+#push-options "--z3rlimit 20 --fuel 1 --ifuel 0 --split_queries always"
+let rec minor_promotion_requests_from_positive
+  (minor: minor_state) (objs: seq U64.t) (idx: nat)
+  : Lemma
+      (requires minor_wf minor /\
+                (forall (j:nat).
+                  idx <= j /\ j < Seq.length objs ==>
+                  Seq.mem (Seq.index objs j) (minor_objects minor)))
+      (ensures
+        MultiAlloc.all_requests_positive
+          (minor_promotion_requests_from minor objs idx))
+      (decreases (Seq.length objs - idx))
+  =
+  if idx >= Seq.length objs then ()
+  else begin
+    let obj = Seq.index objs idx in
+    assert (Seq.mem obj (minor_objects minor));
+    minor_objects_body_bound minor obj;
+    assert (minor_wosize minor obj > 0);
+    let tail_mem (j:nat)
+      : Lemma
+          (requires idx + 1 <= j /\ j < Seq.length objs)
+          (ensures Seq.mem (Seq.index objs j) (minor_objects minor))
+      = ()
+    in
+    assert (forall (j:nat).
+      idx + 1 <= j /\ j < Seq.length objs ==>
+      Seq.mem (Seq.index objs j) (minor_objects minor));
+    minor_promotion_requests_from_positive minor objs (idx + 1)
+  end
+#pop-options
+
+#push-options "--z3rlimit 20 --fuel 1 --ifuel 0 --split_queries always"
+let minor_promotion_requests_positive (minor: minor_state)
+  : Lemma
+      (requires minor_wf minor)
+      (ensures
+        MultiAlloc.all_requests_positive
+          (minor_promotion_requests minor))
+  =
+  let objs = minor_objects minor in
+  let mem_at_index (j:nat)
+    : Lemma
+        (requires 0 <= j /\ j < Seq.length objs)
+        (ensures Seq.mem (Seq.index objs j) (minor_objects minor))
+    =
+    Seq.mem_index (Seq.index objs j) objs
+  in
+  assert (forall (j:nat).
+    0 <= j /\ j < Seq.length objs ==>
+    Seq.mem (Seq.index objs j) (minor_objects minor));
+  minor_promotion_requests_from_positive minor objs 0
+#pop-options
