generational/spec/GC.Gen.PromotionDemand.fsti
@@ -1,0 +1,49 @@
+/// ---------------------------------------------------------------------------
+/// GC.Gen.PromotionDemand -- Conservative minor-promotion allocation demand
+/// ---------------------------------------------------------------------------
+
+module GC.Gen.PromotionDemand
+
+open FStar.Seq
+
+module U64 = FStar.UInt64
+
+open GC.Gen.MinorHeap
+
+module MultiAlloc = GC.Spec.MajorAllocator.MultiAlloc
+
+val minor_promotion_requests_from
+  : minor:minor_state -> objs:seq U64.t -> idx:nat ->
+    GTot (list nat)
+
+val minor_promotion_requests
+  : minor:minor_state -> GTot (list nat)
+
+val minor_promotion_demand
+  : minor:minor_state -> GTot nat
+
+val minor_promotion_demand_eq
+  : minor:minor_state ->
+    Lemma
+      (ensures
+        minor_promotion_demand minor ==
+        MultiAlloc.allocation_list_demand (minor_promotion_requests minor))
+
+val minor_promotion_requests_from_positive
+  : minor:minor_state -> objs:seq U64.t -> idx:nat ->
+    Lemma
+      (requires minor_wf minor /\
+                (forall (j:nat).
+                  idx <= j /\ j < Seq.length objs ==>
+                  Seq.mem (Seq.index objs j) (minor_objects minor)))
+      (ensures
+        MultiAlloc.all_requests_positive
+          (minor_promotion_requests_from minor objs idx))
+
+val minor_promotion_requests_positive
+  : minor:minor_state ->
+    Lemma
+      (requires minor_wf minor)
+      (ensures
+        MultiAlloc.all_requests_positive
+          (minor_promotion_requests minor))
